src/ocaml-output/FStar_TypeChecker_Cfg.ml
@@ -2059,6 +2059,24 @@ let (built_in_primitive_steps : primitive_step FStar_Compiler_Util.psmap) =
               | uu___2 -> FStar_Pervasives_Native.None)
          | uu___1 -> FStar_Pervasives_Native.None)
     | uu___ -> FStar_Pervasives_Native.None in
+  let mixed_ternary_op as_a as_b as_c embed_d f res _norm_cb args =
+    match args with
+    | a1::b1::c1::[] ->
+        let uu___ =
+          let uu___1 = as_a a1 in
+          let uu___2 = as_b b1 in
+          let uu___3 = as_c c1 in (uu___1, uu___2, uu___3) in
+        (match uu___ with
+         | (FStar_Pervasives_Native.Some a2, FStar_Pervasives_Native.Some b2,
+            FStar_Pervasives_Native.Some c2) ->
+             let uu___1 = f res.psc_range a2 b2 c2 in
+             (match uu___1 with
+              | FStar_Pervasives_Native.Some d1 ->
+                  let uu___2 = embed_d res.psc_range d1 in
+                  FStar_Pervasives_Native.Some uu___2
+              | uu___2 -> FStar_Pervasives_Native.None)
+         | uu___1 -> FStar_Pervasives_Native.None)
+    | uu___ -> FStar_Pervasives_Native.None in
   let list_of_string' rng s =
     let name l =
       let uu___ =
@@ -3498,10 +3516,230 @@ let (built_in_primitive_steps : primitive_step FStar_Compiler_Util.psmap) =
                  | uu___3 -> FStar_Pervasives_Native.None))
          (fun body -> body)
          (fun _t -> fun body -> FStar_Pervasives_Native.Some body))) in
+  let array_ops =
+    let of_list_op =
+      let emb_typ t =
+        let uu___ =
+          let uu___1 =
+            FStar_Compiler_Effect.op_Bar_Greater
+              FStar_Parser_Const.cst_seq_lid FStar_Ident.string_of_lid in
+          (uu___1, [t]) in
+        FStar_Syntax_Syntax.ET_app uu___ in
+      let un_lazy t l r =
+        let uu___ =
+          let uu___1 =
+            FStar_Syntax_Util.fvar_const FStar_Parser_Const.cst_of_list_lid in
+          FStar_Syntax_Syntax.mk_Tm_uinst uu___1 [FStar_Syntax_Syntax.U_zero] in
+        let uu___1 =
+          let uu___2 = FStar_Syntax_Syntax.iarg t in
+          let uu___3 = let uu___4 = FStar_Syntax_Syntax.as_arg l in [uu___4] in
+          uu___2 :: uu___3 in
+        FStar_Syntax_Syntax.mk_Tm_app uu___ uu___1 r in
+      (FStar_Parser_Const.cst_of_list_lid, (Prims.of_int (2)), Prims.int_one,
+        (mixed_binary_op
+           (fun uu___ ->
+              match uu___ with
+              | (elt_t, uu___1) -> FStar_Pervasives_Native.Some elt_t)
+           (fun uu___ ->
+              match uu___ with
+              | (l, q) ->
+                  let uu___1 =
+                    arg_as_list FStar_Syntax_Embeddings.e_any (l, q) in
+                  (match uu___1 with
+                   | FStar_Pervasives_Native.Some lst ->
+                       FStar_Pervasives_Native.Some (l, lst)
+                   | uu___2 -> FStar_Pervasives_Native.None))
+           (fun r ->
+              fun uu___ ->
+                match uu___ with
+                | (elt_t, (l, blob)) ->
+                    let uu___1 =
+                      let uu___2 =
+                        let uu___3 =
+                          let uu___4 =
+                            let uu___5 =
+                              let uu___6 =
+                                FStar_Syntax_Embeddings.emb_typ_of
+                                  FStar_Syntax_Embeddings.e_any in
+                              emb_typ uu___6 in
+                            let uu___6 =
+                              FStar_Thunk.mk
+                                (fun uu___7 -> un_lazy elt_t l r) in
+                            (uu___5, uu___6) in
+                          FStar_Syntax_Syntax.Lazy_embedding uu___4 in
+                        let uu___4 =
+                          let uu___5 =
+                            let uu___6 =
+                              FStar_Syntax_Util.fvar_const
+                                FStar_Parser_Const.cst_seq_lid in
+                            FStar_Syntax_Syntax.mk_Tm_uinst uu___6
+                              [FStar_Syntax_Syntax.U_zero] in
+                          let uu___6 =
+                            let uu___7 = FStar_Syntax_Syntax.as_arg elt_t in
+                            [uu___7] in
+                          FStar_Syntax_Syntax.mk_Tm_app uu___5 uu___6 r in
+                        {
+                          FStar_Syntax_Syntax.blob = blob;
+                          FStar_Syntax_Syntax.lkind = uu___3;
+                          FStar_Syntax_Syntax.ltyp = uu___4;
+                          FStar_Syntax_Syntax.rng = r
+                        } in
+                      FStar_Syntax_Syntax.Tm_lazy uu___2 in
+                    FStar_Syntax_Syntax.mk uu___1 r)
+           (fun r ->
+              fun elt_t ->
+                fun uu___ ->
+                  match uu___ with
+                  | (l, lst) ->
+                      let blob = FStar_ConstantTimeSequence.of_list lst in
+                      let uu___1 =
+                        let uu___2 =
+                          let uu___3 = FStar_Compiler_Dyn.mkdyn blob in
+                          (l, uu___3) in
+                        (elt_t, uu___2) in
+                      FStar_Pervasives_Native.Some uu___1)),
+        (FStar_TypeChecker_NBETerm.mixed_binary_op
+           (fun uu___ ->
+              match uu___ with
+              | (elt_t, uu___1) -> FStar_Pervasives_Native.Some elt_t)
+           (fun uu___ ->
+              match uu___ with
+              | (l, q) ->
+                  let uu___1 =
+                    FStar_TypeChecker_NBETerm.arg_as_list
+                      FStar_TypeChecker_NBETerm.e_any (l, q) in
+                  (match uu___1 with
+                   | FStar_Pervasives_Native.None ->
+                       FStar_Pervasives_Native.None
+                   | FStar_Pervasives_Native.Some lst ->
+                       FStar_Pervasives_Native.Some (l, lst)))
+           (fun uu___ ->
+              match uu___ with
+              | (elt_t, (l, blob)) ->
+                  let uu___1 =
+                    let uu___2 =
+                      let uu___3 =
+                        let uu___4 =
+                          let uu___5 =
+                            let uu___6 =
+                              FStar_Syntax_Embeddings.emb_typ_of
+                                FStar_Syntax_Embeddings.e_any in
+                            emb_typ uu___6 in
+                          (blob, uu___5) in
+                        FStar_Pervasives.Inr uu___4 in
+                      let uu___4 =
+                        FStar_Thunk.mk
+                          (fun uu___5 ->
+                             let uu___6 =
+                               let uu___7 =
+                                 let uu___8 =
+                                   FStar_Syntax_Syntax.lid_as_fv
+                                     FStar_Parser_Const.cst_of_list_lid
+                                     FStar_Syntax_Syntax.delta_constant
+                                     FStar_Pervasives_Native.None in
+                                 let uu___9 =
+                                   let uu___10 =
+                                     FStar_TypeChecker_NBETerm.as_arg l in
+                                   [uu___10] in
+                                 (uu___8, [FStar_Syntax_Syntax.U_zero],
+                                   uu___9) in
+                               FStar_TypeChecker_NBETerm.FV uu___7 in
+                             FStar_Compiler_Effect.op_Less_Bar
+                               FStar_TypeChecker_NBETerm.mk_t uu___6) in
+                      (uu___3, uu___4) in
+                    FStar_TypeChecker_NBETerm.Lazy uu___2 in
+                  FStar_Compiler_Effect.op_Less_Bar
+                    FStar_TypeChecker_NBETerm.mk_t uu___1)
+           (fun elt_t ->
+              fun uu___ ->
+                match uu___ with
+                | (l, lst) ->
+                    let blob = FStar_ConstantTimeSequence.of_list lst in
+                    let uu___1 =
+                      let uu___2 =
+                        let uu___3 = FStar_Compiler_Dyn.mkdyn blob in
+                        (l, uu___3) in
+                      (elt_t, uu___2) in
+                    FStar_Pervasives_Native.Some uu___1))) in
+    let arg1_as_elt_t x =
+      FStar_Pervasives_Native.Some (FStar_Pervasives_Native.fst x) in
+    let arg2_as_blob x =
+      let uu___ =
+        let uu___1 =
+          FStar_Syntax_Subst.compress (FStar_Pervasives_Native.fst x) in
+        uu___1.FStar_Syntax_Syntax.n in
+      match uu___ with
+      | FStar_Syntax_Syntax.Tm_lazy
+          { FStar_Syntax_Syntax.blob = blob;
+            FStar_Syntax_Syntax.lkind = FStar_Syntax_Syntax.Lazy_embedding
+              (FStar_Syntax_Syntax.ET_app (head, uu___1), uu___2);
+            FStar_Syntax_Syntax.ltyp = uu___3;
+            FStar_Syntax_Syntax.rng = uu___4;_}
+          when
+          let uu___5 =
+            FStar_Ident.string_of_lid FStar_Parser_Const.cst_seq_lid in
+          head = uu___5 -> FStar_Pervasives_Native.Some blob
+      | uu___1 -> FStar_Pervasives_Native.None in
+    let arg2_as_blob_nbe x =
+      match (FStar_Pervasives_Native.fst x).FStar_TypeChecker_NBETerm.nbe_t
+      with
+      | FStar_TypeChecker_NBETerm.Lazy
+          (FStar_Pervasives.Inr
+           (blob, FStar_Syntax_Syntax.ET_app (head, uu___)), uu___1)
+          when
+          let uu___2 =
+            FStar_Ident.string_of_lid FStar_Parser_Const.cst_seq_lid in
+          head = uu___2 -> FStar_Pervasives_Native.Some blob
+      | uu___ -> FStar_Pervasives_Native.None in
+    let length_op =
+      let embed_int r i = embed_simple FStar_Syntax_Embeddings.e_int r i in
+      let run_op blob =
+        let uu___ =
+          let uu___1 = FStar_Compiler_Dyn.undyn blob in
+          FStar_Compiler_Util.array_length uu___1 in
+        FStar_Pervasives_Native.Some uu___ in
+      (FStar_Parser_Const.cst_length_lid, (Prims.of_int (2)), Prims.int_one,
+        (mixed_binary_op arg1_as_elt_t arg2_as_blob embed_int
+           (fun uu___ -> fun uu___1 -> fun blob -> run_op blob)),
+        (FStar_TypeChecker_NBETerm.mixed_binary_op
+           (fun uu___ ->
+              match uu___ with
+              | (elt_t, uu___1) -> FStar_Pervasives_Native.Some elt_t)
+           arg2_as_blob_nbe
+           (fun i ->
+              FStar_TypeChecker_NBETerm.embed FStar_TypeChecker_NBETerm.e_int
+                bogus_cbs i) (fun uu___ -> fun blob -> run_op blob))) in
+    let index_op =
+      (FStar_Parser_Const.cst_index_lid, (Prims.of_int (3)), Prims.int_one,
+        (mixed_ternary_op arg1_as_elt_t arg2_as_blob arg_as_int
+           (fun r -> fun tm -> tm)
+           (fun r ->
+              fun _t ->
+                fun blob ->
+                  fun i ->
+                    let uu___ =
+                      let uu___1 = FStar_Compiler_Dyn.undyn blob in
+                      FStar_Compiler_Util.array_index uu___1 i in
+                    FStar_Pervasives_Native.Some uu___)),
+        (FStar_TypeChecker_NBETerm.mixed_ternary_op
+           (fun uu___ ->
+              match uu___ with
+              | (elt_t, uu___1) -> FStar_Pervasives_Native.Some elt_t)
+           arg2_as_blob_nbe FStar_TypeChecker_NBETerm.arg_as_int
+           (fun tm -> tm)
+           (fun _t ->
+              fun blob ->
+                fun i ->
+                  let uu___ =
+                    let uu___1 = FStar_Compiler_Dyn.undyn blob in
+                    FStar_Compiler_Util.array_index uu___1 i in
+                  FStar_Pervasives_Native.Some uu___))) in
+    [of_list_op; length_op; index_op] in
   let strong_steps =
     FStar_Compiler_List.map (as_primitive_step true)
       (FStar_Compiler_List.op_At basic_ops
-         (FStar_Compiler_List.op_At bounded_arith_ops [reveal_hide])) in
+         (FStar_Compiler_List.op_At bounded_arith_ops
+            (FStar_Compiler_List.op_At [reveal_hide] array_ops))) in
   let weak_steps = FStar_Compiler_List.map (as_primitive_step false) weak_ops in
   FStar_Compiler_Effect.op_Less_Bar prim_from_list
     (FStar_Compiler_List.op_At strong_steps weak_steps)
