src/typechecker/FStar.TypeChecker.NBETerm.fst
@@ -499,6 +499,25 @@ let e_list (ea:embedding 'a) =
     in
     mk_emb em un (lid_as_typ PC.list_lid [U_zero] [as_arg (type_of ea)]) etyp
 
+let e_array (ea:embedding 'a)
+  : embedding (FStar.ConstantTimeSequence.seq 'a)
+  = let etyp = ET_app(PC.cst_seq_lid |> Ident.string_of_lid, [ea.emb_typ]) in
+    let t_seq_a =
+        let t_seq = S.mk_Tm_uinst (U.fvar_const PC.cst_seq_lid) [U_zero] in
+        S.mk_Tm_app t_seq [S.as_arg S.tun] Range.dummyRange
+    in
+    let em cb (l:FStar.ConstantTimeSequence.seq 'a) : t =
+      let li = { blob = FStar.Compiler.Dyn.mkdyn l; lkind = Lazy_native_array; ltyp = t_seq_a; rng = Range.dummyRange } in
+      let rec thunk () = mk_t (Lazy (Inl li, Thunk.mk thunk)) in
+      thunk ()
+    in
+    let un cb (trm:t) : option (FStar.ConstantTimeSequence.seq 'a) =
+      match trm.nbe_t with
+      | Lazy (Inl li, _) -> Some (FStar.Compiler.Dyn.undyn li.blob)
+      | _ -> None
+    in
+    mk_emb em un (lid_as_typ PC.cst_seq_lid [U_zero] [as_arg (type_of ea)]) etyp
+  
 let e_string_list = e_list e_string
 
 let e_arrow (ea:embedding 'a) (eb:embedding 'b) : embedding ('a -> 'b) =
@@ -669,6 +688,24 @@ let mixed_binary_op (as_a : arg -> option 'a) (as_b : arg -> option 'b)
                 | Some a, Some b ->
                   (match f a b with
                    | Some c -> Some (embed_c c)
+                   | _ -> None)
+                | _ -> None
+                end
+             | _ -> None
+
+let mixed_ternary_op (as_a : arg -> option 'a)
+                     (as_b : arg -> option 'b)
+                     (as_c : arg -> option 'c)                     
+                     (embed_d : 'd -> t) 
+                     (f : 'a -> 'b -> 'c -> option 'd)
+                     (args : args) : option t =
+             match args with
+             | [a;b;c] ->
+                begin
+                match as_a a, as_b b, as_c c with
+                | Some a, Some b, Some c ->
+                  (match f a b c with
+                   | Some d -> Some (embed_d d)
                    | _ -> None)
                 | _ -> None
                 end
