ulib/FStar.ConstantTimeSequence.fsti
@@ -1,0 +1,9 @@
+module FStar.ConstantTimeSequence.Base
+
+val seq (a:Type u#a) : Type u#a
+
+val of_list (#a:Type u#a) (l:list a) : Tot (seq a)
+
+val length (#a:Type) (s:seq a) : Tot nat
+
+val index (#a:Type) (s:seq a) (i:nat { i < length s }) : Tot a
